有
$$
\boldsymbol{X}_k=\boldsymbol{A}\boldsymbol{X}_{k-1}+\boldsymbol{B}\boldsymbol{u}_{k-1}+\boldsymbol{w}_{k-1}\quad,\quad p(\boldsymbol{w})\textasciitilde N(0,\boldsymbol{Q})
$$
$$
\boldsymbol{Z}_k=\boldsymbol{H}\boldsymbol{X}_k+\boldsymbol{v}_k\quad,\quad p(\boldsymbol{v})\textasciitilde N(0,\boldsymbol{R})
$$
先验估计：
$$
\hat{\boldsymbol{X}}_k^-=\boldsymbol{A}\hat{\boldsymbol{X}}_{k-1}+\boldsymbol{B}\boldsymbol{u}_{k-1}
$$
后验估计：
$$
\hat{\boldsymbol{X}_k}=\hat{\boldsymbol{X}}_k^-+K_k(\boldsymbol{Z}_k-\boldsymbol{H}\hat{\boldsymbol{X}}_k^-)
$$
卡尔曼增益：
$$
K_k=\frac{\boldsymbol{P_k^-}\boldsymbol{H}^T}{\boldsymbol{HP}_k^-\boldsymbol{H}^T+\boldsymbol{R}}
$$
以上仅$\boldsymbol{P}_k^-$未知
# 推导
## 先验误差协方差
$$
\boldsymbol{P}_k^-=E\left[\boldsymbol{e}_k^-{\boldsymbol{e}_k^-}^T\right]
$$
展开
$$
\begin{align}
\boldsymbol{e}_k^-&=\boldsymbol{X}_k-\hat{\boldsymbol{X}}_k^-\\
&=\boldsymbol{A}\boldsymbol{X}_{k-1}+\boldsymbol{B}\boldsymbol{u}_k+\boldsymbol{w}_{k-1}-\boldsymbol{A}\hat{\boldsymbol{X}}_{k-1}-\boldsymbol{B}\boldsymbol{u}_{k-1}\\
&=\boldsymbol{A}(\boldsymbol{X}_{k-1}-\hat{\boldsymbol{X}}_{k-1})+\boldsymbol{w}_{k-1}\\
&=\boldsymbol{A}\boldsymbol{e}_{k-1}+\boldsymbol{w}_{k-1}
\end{align}
$$
代入
$$
\begin{align}
\boldsymbol{P}_k^-&=E\left[\boldsymbol{e}_k^-{\boldsymbol{e}_k^-}^T\right]\\
&=E\left[(\boldsymbol{Ae}_{k-1}+\boldsymbol{w}_{k-1})(\boldsymbol{Ae}_{k-1}+\boldsymbol{w}_{k-1})^T\right]\\
&=E\left[(\boldsymbol{Ae}_{k-1}+\boldsymbol{w}_{k-1})(\boldsymbol{e}_{k-1}^T\boldsymbol{A}^T+\boldsymbol{w}_{k-1}^T)\right]\\
&=E\left[\boldsymbol{Ae}_{k-1}\boldsymbol{e}_{k-1}^T\boldsymbol{A}^T\right]+E\left[\boldsymbol{Ae}_{k-1}\boldsymbol{w}_{k-1}^T\right]+E\left[\boldsymbol{w}_{k-1}\boldsymbol{e}_{k-1}^T\boldsymbol{A}^T\right]+E\left[\boldsymbol{w}_{k-1}\boldsymbol{w}_{k-1}^T\right]\\
&=\boldsymbol{A}E\left[\boldsymbol{e}_{k-1}\boldsymbol{e}_{k-1}^T\right]\boldsymbol{A}^T+E\left[\boldsymbol{w}_{k-1}\boldsymbol{w}_{k-1}^T\right]\\
&=\boldsymbol{A}\boldsymbol{P}_{k-1}\boldsymbol{A}^T+\boldsymbol{Q}
\end{align}
$$
## 后验误差协方差
$$
\begin{align}
\boldsymbol{P}_k&=\boldsymbol{P}_k^--K_k\boldsymbol{H}\boldsymbol{P}_k^--\boldsymbol{P}_k^-\boldsymbol{H}^TK_k^T+K_k\boldsymbol{H}\boldsymbol{P}_k^-\boldsymbol{H}^TK_k^T+K_k\boldsymbol{R}K_k^T\\
&\xlongequal{K_k=\frac{\boldsymbol{P_k^-}\boldsymbol{H}^T}{\boldsymbol{HP}_k^-\boldsymbol{H}^T+\boldsymbol{R}}}\boldsymbol{P}_k^--K_k\boldsymbol{H}\boldsymbol{P}_k^-\\
&=(\boldsymbol{I}-K_k\boldsymbol{H})\boldsymbol{P}_k^-
\end{align}
$$

# 求解步骤
## 预测
1. 先验：$\hat{\boldsymbol{X}}_k^-=\boldsymbol{A}\hat{\boldsymbol{X}}_{k-1}+\boldsymbol{B}\boldsymbol{u}_{k-1}$
2. 先验误差协方差：$\boldsymbol{P}_k^-=\boldsymbol{A}\boldsymbol{P}_{k-1}\boldsymbol{A}^T+\boldsymbol{Q}$
## 校正
1. 卡尔曼增益：$K_k=\frac{\boldsymbol{P_k^-}\boldsymbol{H}^T}{\boldsymbol{HP}_k^-\boldsymbol{H}^T+\boldsymbol{R}}$
2. 后验估计：$\hat{\boldsymbol{X}_k}=\hat{\boldsymbol{X}}_k^-+K_k(\boldsymbol{Z}_k-\boldsymbol{H}\hat{\boldsymbol{X}}_k^-)$
3. 更新误差协方差：$\boldsymbol{P}_k=(\boldsymbol{I}-K_k\boldsymbol{H})\boldsymbol{P}_k^-$